split lemmas and specs

ver3_less_complex/Invariants.dfy
@@ -1,107 +1,16 @@
 include "Type.dfy"
-include "System.dfy"
 include "Auxilarily.dfy"
 
 
 module M_Invariants {
     import opened M_SpecTypes
-    import opened M_System
     import opened M_AuxilarilyFunc
 
-
-
-    /**
-     * Invariant: Constant fields kept by the system, e.g. Node counts(Honest & Byzantine), Node role(Honest always be honest?)
-     */
-    ghost predicate Inv_Constant_Fields(ss : SystemState)
-    {
-      && ss.adversary.byz_nodes == M_SpecTypes.Adversary_Nodes
-      && ss.nodeStates.Keys == M_SpecTypes.All_Nodes
+    predicate Inv_Node_Constraint()
+    {   
+        && |M_SpecTypes.All_Nodes| > 0
+        && |Adversary_Nodes| <= f(|All_Nodes|)
+        && M_SpecTypes.Honest_Nodes * M_SpecTypes.Adversary_Nodes == {}
     }
-
-
-    /**
-     * Invariant: Each honest node are forced to vote PROPOSAL only one time at the same view. See Page(6): PROOF of Lemma 1
-     */
-    ghost predicate Inv_Honest_Node_Only_Vote_One_Proposal_At_Same_View(ss : SystemState)
-    {
-        forall r | IsHonest(ss, r) ::
-            var msgReceived := ss.nodeStates[r].msgReceived;
-            forall m1, m2 | 
-                            && m1 in msgReceived
-                            && m2 in msgReceived
-                            && m1.mType == MT_Prepare
-                            && m2.mType == MT_Prepare
-                            && m1.partialSig.Signature?
-                            && m2.partialSig.Signature?
-                            && m1.partialSig.signer == m2.partialSig.signer
-                            && IsHonest(ss, m1.partialSig.signer)
-                            && m1.viewNum == m2.viewNum
-                          ::
-                            && m1 == m2
-                            && m1.partialSig.block == m2.partialSig.block
-    }
-
-
-    /**
-     * Invariant: Each honest node are forced to vote only one PREPARE message from leader at the same view. See Page(6): PROOF of Lemma 1
-     */
-    ghost predicate Inv_Honest_Node_Only_Vote_One_Prepare_At_Same_View(ss : SystemState)
-    {
-        forall r | IsHonest(ss, r) ::
-            var msgReceived := ss.nodeStates[r].msgReceived;
-            forall m1, m2 | 
-                            && m1 in msgReceived
-                            && m2 in msgReceived
-                            && m1.mType == MT_PreCommit
-                            && m2.mType == MT_PreCommit
-                            && m1.partialSig.Signature?
-                            && m2.partialSig.Signature?
-                            && m1.partialSig.signer == m2.partialSig.signer
-                            && IsHonest(ss, m1.partialSig.signer)
-                            && m1.viewNum == m2.viewNum
-                          ::
-                            && m1 == m2
-                            && m1.partialSig.block == m2.partialSig.block
-    }
-
-
-    /**
-     * Invariant: Each honest node are forced to vote only one PRECOMMIT message from leader at the same view. See Page(6): PROOF of Lemma 1
-     */
-    ghost predicate Inv_Honest_Node_Only_Vote_One_PreCommit_At_Same_View(ss : SystemState)
-    {
-        forall r | IsHonest(ss, r) ::
-            var msgReceived := ss.nodeStates[r].msgReceived;
-            forall m1, m2 | 
-                            && m1 in msgReceived
-                            && m2 in msgReceived
-                            && m1.mType == MT_Commit
-                            && m2.mType == MT_Commit
-                            && m1.partialSig.Signature?
-                            && m2.partialSig.Signature?
-                            && m1.partialSig.signer == m2.partialSig.signer
-                            && IsHonest(ss, m1.partialSig.signer)
-                            && m1.viewNum == m2.viewNum
-                          ::
-                            && m1 == m2
-                            && m1.partialSig.block == m2.partialSig.block
-    }
-
-    ghost predicate Inv_Honest_Node_Commit_Not_Conflict_Block(ss : SystemState)
-    {
-        forall r1, r2 | 
-                        && IsHonest(ss, r1)
-                        && IsHonest(ss, r2)
-                      ::
-                        && ss.nodeStates[r1].commitQC.Cert?
-                        && ss.nodeStates[r2].commitQC.Cert?
-                        && ss.nodeStates[r1].commitQC.block.Block?
-                        && ss.nodeStates[r2].commitQC.block.Block?
-                        && NoConflict(ss.nodeStates[r1].commitQC.block, ss.nodeStates[r2].commitQC.block)   //TODO: define block confliction
-            
-    }
-
-    // ghost predicate Inv_
 
 }
