ver3_less_complex/System.dfy
@@ -2,6 +2,8 @@ include "Type.dfy"
 include "Adversary.dfy"
 include "Replica.dfy"
 include "Auxilarily.dfy"
+include "Axioms.dfy"
+include "Invariants.dfy"
 
 module M_System {
 
@@ -9,6 +11,8 @@ module M_System {
     import opened M_Replica
     import opened M_Adversary
     import opened M_AuxilarilyFunc
+    import opened M_Axiom
+    import opened M_Invariants
 
     /**
      * Definition of a system state
@@ -32,170 +36,192 @@ module M_System {
         // r in M_SpecTypes.Honest_Nodes
     }
 
-    predicate Inv_Node_Constraint(ss : SystemState)
+    predicate Inv_Node_System(ss : SystemState)
     {
-        && |M_SpecTypes.All_Nodes| > 0
-        && |Adversary_Nodes| <= f(|All_Nodes|)
-        && M_SpecTypes.Honest_Nodes * M_SpecTypes.Adversary_Nodes == {}
+        && Inv_Node_Constraint()
         && ss.nodeStates.Keys == M_SpecTypes.All_Nodes
         && ss.adversary.byz_nodes == M_SpecTypes.Adversary_Nodes
     }
 
     ghost predicate ValidSystemState(ss : SystemState)
     {
-        && Inv_Node_Constraint(ss)
+        NoOuterClient();
+        && Inv_Node_System(ss)
         && (forall replica | replica in ss.nodeStates.Keys :: ss.nodeStates[replica].msgSent <= ss.msgSent)
         && (forall replica | IsHonest(ss, replica) :: ValidReplicaState(ss.nodeStates[replica]))
         && (forall replica | IsHonest(ss, replica) :: ss.nodeStates[replica].msgReceived <= ss.msgSent)
-        // && forall m | m in ss.msgSent
-        //            :: (exists r | r in ss.nodeStates.Keys
-        //                        :: m in ss.nodeStates[r].msgSent)
+
+        // && forall m | m in ss.msgSent && IsHonest(ss, m.sender)
+        //            :: m in ss.nodeStates[m.sender].msgSent
     }
 
-    lemma LemmaInitialSystemStateHoldsValidity(ss : SystemState)
-    requires SystemInit(ss)
-    ensures ValidSystemState(ss)
-    {
+    // lemma LemmaInitialSystemStateHoldsValidity(ss : SystemState)
+    // requires SystemInit(ss)
+    // ensures ValidSystemState(ss)
+    // {
 
-    }
+    // }
 
-    lemma LemmaSystemTransitionHoldsValidity(ss : SystemState, ss' : SystemState)
-    requires ValidSystemState(ss)
-    requires SystemNext(ss, ss')
-    ensures ValidSystemState(ss')
-    {
-        // Prove a valid state after system transition will still be valid
-        if ss == ss' {
-            assert ValidSystemState(ss');
-        }
-        else {
-            // assert false;
-            forall replica, msgReceivedByNodes, msgSentByNodes
-                    | && msgReceivedByNodes <= ss.msgSent
-                      && SystemNextByOneReplica(ss, ss', replica, msgReceivedByNodes, msgSentByNodes)
-            ensures ValidSystemState(ss') {
-                LemmaSystemNextByOneReplicaIsValid(ss, ss', replica, msgReceivedByNodes, msgSentByNodes);
-            }
-        }
-    }
+    // lemma LemmaSystemTransitionHoldsValidity(ss : SystemState, ss' : SystemState)
+    // requires ValidSystemState(ss)
+    // requires SystemNext(ss, ss')
+    // ensures ValidSystemState(ss')
+    // {
+    //     // Prove a valid state after system transition will still be valid
+    //     if ss == ss' {
+    //         assert ValidSystemState(ss');
+    //     }
+    //     else {
+    //         // assert false;
+    //         forall replica, msgReceivedByNodes, msgSentByNodes
+    //                 | && msgReceivedByNodes <= ss.msgSent
+    //                   && SystemNextByOneReplica(ss, ss', replica, msgReceivedByNodes, msgSentByNodes)
+    //         ensures ValidSystemState(ss') {
+    //             LemmaSystemNextByOneReplicaIsValid(ss, ss', replica, msgReceivedByNodes, msgSentByNodes);
+    //         }
+    //     }
+    // }
 
-    lemma LemmaReplicaMsgReceivedMustBeSent(
-        ss : SystemState,
-        ss' : SystemState
-    )
-    requires ValidSystemState(ss)
-    requires SystemNext(ss, ss')
-    ensures forall r | IsHonest(ss', r) :: ss'.nodeStates[r].msgReceived <= ss'.msgSent
-    {
-        if ss == ss' {
+    // lemma LemmaReplicaMsgReceivedMustBeSent(
+    //     ss : SystemState,
+    //     ss' : SystemState
+    // )
+    // requires ValidSystemState(ss)
+    // requires SystemNext(ss, ss')
+    // ensures forall r | IsHonest(ss', r) :: ss'.nodeStates[r].msgReceived <= ss'.msgSent
+    // {
+    //     if ss == ss' {
 
-        }
-        else {
-            // assert false;
-            var replica, msgReceivedByNodes, msgSentByNodes
-                   :|   && msgReceivedByNodes <= ss.msgSent
-                        && SystemNextByOneReplica(ss, ss', replica, msgReceivedByNodes, msgSentByNodes);
-            LemmaSystemNextByOneReplicaIsValid(ss, ss', replica, msgReceivedByNodes, msgSentByNodes);
-        }
-    }
+    //     }
+    //     else {
+    //         // assert false;
+    //         var replica, msgReceivedByNodes, msgSentByNodes
+    //                :|   && msgReceivedByNodes <= ss.msgSent
+    //                     && SystemNextByOneReplica(ss, ss', replica, msgReceivedByNodes, msgSentByNodes);
+    //         LemmaSystemNextByOneReplicaIsValid(ss, ss', replica, msgReceivedByNodes, msgSentByNodes);
+    //     }
+    // }
 
-    lemma LemmaInvNodeInSystemNextByOneReplica(
-        ss : SystemState, 
-        ss' : SystemState, 
-        replica : Address,
-        inMsg : set<Msg>,
-        outMsg : set<Msg>)
-    requires ValidSystemState(ss)
-    requires inMsg <= ss.msgSent
-    requires SystemNextByOneReplica(ss, ss', replica, inMsg, outMsg)
-    ensures Inv_Node_Constraint(ss')
-    {
+    // lemma LemmaInvNodeInSystemNextByOneReplica(
+    //     ss : SystemState, 
+    //     ss' : SystemState, 
+    //     replica : Address,
+    //     inMsg : set<Msg>,
+    //     outMsg : set<Msg>)
+    // requires ValidSystemState(ss)
+    // requires inMsg <= ss.msgSent
+    // requires SystemNextByOneReplica(ss, ss', replica, inMsg, outMsg)
+    // ensures Inv_Node_System(ss')
+    // {
 
-    }
+    // }
 
-    lemma LemmaHonestReplicaIsValidInSystemNextByOneReplica(
-        ss : SystemState, 
-        ss' : SystemState, 
-        replica : Address,
-        inMsg : set<Msg>,
-        outMsg : set<Msg>)
-    requires ValidSystemState(ss)
-    requires inMsg <= ss.msgSent
-    requires SystemNextByOneReplica(ss, ss', replica, inMsg, outMsg)
-    ensures forall r | IsHonest(ss', r) :: ValidReplicaState(ss'.nodeStates[r])
-    {
-        if IsHonest(ss, replica) {
-            LemmaReplicaNextIsValid(ss.nodeStates[replica],
-                                    inMsg,
-                                    ss'.nodeStates[replica],
-                                    outMsg);
-        }
-    }
+    // lemma LemmaHonestReplicaIsValidInSystemNextByOneReplica(
+    //     ss : SystemState, 
+    //     ss' : SystemState, 
+    //     replica : Address,
+    //     inMsg : set<Msg>,
+    //     outMsg : set<Msg>)
+    // requires ValidSystemState(ss)
+    // requires inMsg <= ss.msgSent
+    // requires SystemNextByOneReplica(ss, ss', replica, inMsg, outMsg)
+    // ensures forall r | IsHonest(ss', r) :: ValidReplicaState(ss'.nodeStates[r])
+    // {
+    //     if IsHonest(ss, replica) {
+    //         LemmaReplicaNextIsValid(ss.nodeStates[replica],
+    //                                 inMsg,
+    //                                 ss'.nodeStates[replica],
+    //                                 outMsg);
+    //     }
+    // }
 
-    lemma LemmaHonestReplicaMsgReceivedIsSubsetOfSystemMsgSentInSystemNextByOneReplica(
-        ss : SystemState, 
-        ss' : SystemState, 
-        replica : Address,
-        inMsg : set<Msg>,
-        outMsg : set<Msg>)
-    requires ValidSystemState(ss)
-    requires inMsg <= ss.msgSent
-    requires SystemNextByOneReplica(ss, ss', replica, inMsg, outMsg)
-    ensures forall r | IsHonest(ss', r) :: ss'.nodeStates[r].msgReceived <= ss'.msgSent
-    {
-        if IsHonest(ss, replica) {
-            var rState := ss.nodeStates[replica];
-            var rState' := ss'.nodeStates[replica];
-            LemmaMsgRelationInReplicaNext(rState, inMsg, rState', outMsg);
-        }
-    }
+    // lemma LemmaHonestSentMsgCapturedBySystemInSystemNextByOneReplica(
+    //         ss : SystemState, 
+    //         ss' : SystemState, 
+    //         replica : Address,
+    //         inMsg : set<Msg>,
+    //         outMsg : set<Msg>)
+    // requires ValidSystemState(ss)
+    // requires inMsg <= ss.msgSent
+    // requires SystemNextByOneReplica(ss, ss', replica, inMsg, outMsg)
+    // ensures forall m | m in outMsg && IsHonest(ss', m.sender) :: m in ss'.nodeStates[m.sender].msgSent
+    // {
+    //     if IsHonest(ss, replica) {
+    //         var r := ss.nodeStates[replica];
+    //         var r' := ss'.nodeStates[replica];
+    //         // LemmaMsgRelationInReplicaNext(rState, inMsg, rState', outMsg);
+    //         LemmaMsgSentWithBySameReplicaInReplicaNext(r, inMsg, r', outMsg);
+    //         assert forall m | m in outMsg :: m.sender == replica;
+    //     }
+    //     // else {
+            
+    //     // }
+    // }
 
-    lemma LemmaReplicaMsgSentIsSubsetOfSystemMsgSentInSystemNextByOneReplica(
-        ss : SystemState, 
-        ss' : SystemState, 
-        replica : Address,
-        inMsg : set<Msg>,
-        outMsg : set<Msg>)
-    requires ValidSystemState(ss)
-    requires inMsg <= ss.msgSent
-    requires SystemNextByOneReplica(ss, ss', replica, inMsg, outMsg)
-    ensures forall r | r in ss'.nodeStates.Keys :: ss'.nodeStates[r].msgSent <= ss'.msgSent
-    {
-        if IsHonest(ss, replica) {
-            var rState := ss.nodeStates[replica];
-            var rState' := ss'.nodeStates[replica];
-            LemmaMsgRelationInReplicaNext(rState, inMsg, rState', outMsg);
-            assert rState'.msgSent <= ss'.msgSent;
-        }
-        else {
-            forall r_byz | r_byz in ss.adversary.byz_nodes
-            ensures ss'.nodeStates[r_byz].msgSent <= ss'.msgSent {
-                var byzState := ss.nodeStates[r_byz];
-                var byzState' := ss'.nodeStates[r_byz];
-                // assert forall r | r in ss.nodeStates.Keys :: ss.nodeStates[r].msgSent <= ss.msgSent by {
-                //     assert ValidSystemState(ss);
-                // }
-                assert byzState'.msgSent <= ss'.msgSent;
-            }
-        }
-    }
+    // lemma LemmaHonestReplicaMsgReceivedIsSubsetOfSystemMsgSentInSystemNextByOneReplica(
+    //     ss : SystemState, 
+    //     ss' : SystemState, 
+    //     replica : Address,
+    //     inMsg : set<Msg>,
+    //     outMsg : set<Msg>)
+    // requires ValidSystemState(ss)
+    // requires inMsg <= ss.msgSent
+    // requires SystemNextByOneReplica(ss, ss', replica, inMsg, outMsg)
+    // ensures forall r | IsHonest(ss', r) :: ss'.nodeStates[r].msgReceived <= ss'.msgSent
+    // {
+    //     if IsHonest(ss, replica) {
+    //         var rState := ss.nodeStates[replica];
+    //         var rState' := ss'.nodeStates[replica];
+    //         LemmaMsgRelationInReplicaNext(rState, inMsg, rState', outMsg);
+    //     }
+    // }
 
-    lemma LemmaSystemNextByOneReplicaIsValid(
-        ss : SystemState, 
-        ss' : SystemState, 
-        replica : Address,
-        inMsg : set<Msg>,
-        outMsg : set<Msg>)
-    requires ValidSystemState(ss)
-    requires inMsg <= ss.msgSent
-    requires SystemNextByOneReplica(ss, ss', replica, inMsg, outMsg)
-    ensures ValidSystemState(ss')
-    {
-        LemmaInvNodeInSystemNextByOneReplica(ss, ss', replica, inMsg, outMsg);
-        LemmaReplicaMsgSentIsSubsetOfSystemMsgSentInSystemNextByOneReplica(ss, ss', replica, inMsg, outMsg);
-        LemmaHonestReplicaIsValidInSystemNextByOneReplica(ss, ss', replica, inMsg, outMsg);
-        LemmaHonestReplicaMsgReceivedIsSubsetOfSystemMsgSentInSystemNextByOneReplica(ss, ss', replica, inMsg, outMsg);
-    }
+    // lemma LemmaReplicaMsgSentIsSubsetOfSystemMsgSentInSystemNextByOneReplica(
+    //     ss : SystemState, 
+    //     ss' : SystemState, 
+    //     replica : Address,
+    //     inMsg : set<Msg>,
+    //     outMsg : set<Msg>)
+    // requires ValidSystemState(ss)
+    // requires inMsg <= ss.msgSent
+    // requires SystemNextByOneReplica(ss, ss', replica, inMsg, outMsg)
+    // ensures forall r | r in ss'.nodeStates.Keys :: ss'.nodeStates[r].msgSent <= ss'.msgSent
+    // {
+    //     if IsHonest(ss, replica) {
+    //         var rState := ss.nodeStates[replica];
+    //         var rState' := ss'.nodeStates[replica];
+    //         LemmaMsgRelationInReplicaNext(rState, inMsg, rState', outMsg);
+    //         assert rState'.msgSent <= ss'.msgSent;
+    //     }
+    //     else {
+    //         forall r_byz | r_byz in ss.adversary.byz_nodes
+    //         ensures ss'.nodeStates[r_byz].msgSent <= ss'.msgSent {
+    //             var byzState := ss.nodeStates[r_byz];
+    //             var byzState' := ss'.nodeStates[r_byz];
+    //             // assert forall r | r in ss.nodeStates.Keys :: ss.nodeStates[r].msgSent <= ss.msgSent by {
+    //             //     assert ValidSystemState(ss);
+    //             // }
+    //             assert byzState'.msgSent <= ss'.msgSent;
+    //         }
+    //     }
+    // }
+
+    // lemma LemmaSystemNextByOneReplicaIsValid(
+    //     ss : SystemState, 
+    //     ss' : SystemState, 
+    //     replica : Address,
+    //     inMsg : set<Msg>,
+    //     outMsg : set<Msg>)
+    // requires ValidSystemState(ss)
+    // requires inMsg <= ss.msgSent
+    // requires SystemNextByOneReplica(ss, ss', replica, inMsg, outMsg)
+    // ensures ValidSystemState(ss')
+    // {
+    //     LemmaInvNodeInSystemNextByOneReplica(ss, ss', replica, inMsg, outMsg);
+    //     LemmaReplicaMsgSentIsSubsetOfSystemMsgSentInSystemNextByOneReplica(ss, ss', replica, inMsg, outMsg);
+    //     LemmaHonestReplicaIsValidInSystemNextByOneReplica(ss, ss', replica, inMsg, outMsg);
+    //     LemmaHonestReplicaMsgReceivedIsSubsetOfSystemMsgSentInSystemNextByOneReplica(ss, ss', replica, inMsg, outMsg);
+    // }
 
     /**
      * Definition of initial state of system
@@ -203,8 +229,8 @@ module M_System {
     ghost predicate SystemInit(ss : SystemState)
     // ensures ValidSystemState(ss)
     {
-        && Inv_Node_Constraint(ss)
-        && ss.msgSent == {getInitialMsg()}
+        && Inv_Node_System(ss)
+        && ss.msgSent == getMultiInitialMsg(ss.nodeStates.Keys)
         && ss.nodeStates.Keys == M_SpecTypes.All_Nodes
         && (forall r | r in ss.nodeStates :: ReplicaInit(ss.nodeStates[r], r))
         && AdversaryInit(ss.adversary)
