ver3_less_complex/Lemmas_System.dfy
@@ -1,0 +1,180 @@
+include "Type.dfy"
+include "Replica.dfy"
+include "System.dfy"
+include "Lemmas_Replica.dfy"
+
+module M_Lemmas_System {
+    import opened M_SpecTypes
+    import opened M_Replica
+    import opened M_System
+    import opened M_Lemmas_Replica
+
+    lemma LemmaInitialSystemStateHoldsValidity(ss : SystemState)
+    requires SystemInit(ss)
+    ensures ValidSystemState(ss)
+    {
+
+    }
+
+    lemma LemmaSystemTransitionHoldsValidity(ss : SystemState, ss' : SystemState)
+    requires ValidSystemState(ss)
+    requires SystemNext(ss, ss')
+    ensures ValidSystemState(ss')
+    {
+        // Prove a valid state after system transition will still be valid
+        if ss == ss' {
+            assert ValidSystemState(ss');
+        }
+        else {
+            // assert false;
+            forall replica, msgReceivedByNodes, msgSentByNodes
+                    | && msgReceivedByNodes <= ss.msgSent
+                      && SystemNextByOneReplica(ss, ss', replica, msgReceivedByNodes, msgSentByNodes)
+            ensures ValidSystemState(ss') {
+                LemmaSystemNextByOneReplicaIsValid(ss, ss', replica, msgReceivedByNodes, msgSentByNodes);
+            }
+        }
+    }
+
+    lemma LemmaReplicaMsgReceivedMustBeSent(
+        ss : SystemState,
+        ss' : SystemState
+    )
+    requires ValidSystemState(ss)
+    requires SystemNext(ss, ss')
+    ensures forall r | IsHonest(ss', r) :: ss'.nodeStates[r].msgReceived <= ss'.msgSent
+    {
+        if ss == ss' {
+
+        }
+        else {
+            // assert false;
+            var replica, msgReceivedByNodes, msgSentByNodes
+                   :|   && msgReceivedByNodes <= ss.msgSent
+                        && SystemNextByOneReplica(ss, ss', replica, msgReceivedByNodes, msgSentByNodes);
+            LemmaSystemNextByOneReplicaIsValid(ss, ss', replica, msgReceivedByNodes, msgSentByNodes);
+        }
+    }
+
+    lemma LemmaInvNodeInSystemNextByOneReplica(
+        ss : SystemState, 
+        ss' : SystemState, 
+        replica : Address,
+        inMsg : set<Msg>,
+        outMsg : set<Msg>)
+    requires ValidSystemState(ss)
+    requires inMsg <= ss.msgSent
+    requires SystemNextByOneReplica(ss, ss', replica, inMsg, outMsg)
+    ensures Inv_Node_System(ss')
+    {
+
+    }
+
+    lemma LemmaHonestReplicaIsValidInSystemNextByOneReplica(
+        ss : SystemState, 
+        ss' : SystemState, 
+        replica : Address,
+        inMsg : set<Msg>,
+        outMsg : set<Msg>)
+    requires ValidSystemState(ss)
+    requires inMsg <= ss.msgSent
+    requires SystemNextByOneReplica(ss, ss', replica, inMsg, outMsg)
+    ensures forall r | IsHonest(ss', r) :: ValidReplicaState(ss'.nodeStates[r])
+    {
+        if IsHonest(ss, replica) {
+            LemmaReplicaNextIsValid(ss.nodeStates[replica],
+                                    inMsg,
+                                    ss'.nodeStates[replica],
+                                    outMsg);
+        }
+    }
+
+    lemma LemmaHonestSentMsgCapturedBySystemInSystemNextByOneReplica(
+            ss : SystemState, 
+            ss' : SystemState, 
+            replica : Address,
+            inMsg : set<Msg>,
+            outMsg : set<Msg>)
+    requires ValidSystemState(ss)
+    requires inMsg <= ss.msgSent
+    requires SystemNextByOneReplica(ss, ss', replica, inMsg, outMsg)
+    ensures forall m | m in outMsg && IsHonest(ss', m.sender) :: m in ss'.nodeStates[m.sender].msgSent
+    {
+        if IsHonest(ss, replica) {
+            var r := ss.nodeStates[replica];
+            var r' := ss'.nodeStates[replica];
+            // LemmaMsgRelationInReplicaNext(rState, inMsg, rState', outMsg);
+            LemmaMsgSentWithBySameReplicaInReplicaNext(r, inMsg, r', outMsg);
+            assert r'.id == replica;
+            assert forall m | m in outMsg :: m.sender == replica;
+        }
+        else {
+            
+        }
+    }
+
+    lemma LemmaHonestReplicaMsgReceivedIsSubsetOfSystemMsgSentInSystemNextByOneReplica(
+        ss : SystemState, 
+        ss' : SystemState, 
+        replica : Address,
+        inMsg : set<Msg>,
+        outMsg : set<Msg>)
+    requires ValidSystemState(ss)
+    requires inMsg <= ss.msgSent
+    requires SystemNextByOneReplica(ss, ss', replica, inMsg, outMsg)
+    ensures forall r | IsHonest(ss', r) :: ss'.nodeStates[r].msgReceived <= ss'.msgSent
+    {
+        if IsHonest(ss, replica) {
+            var rState := ss.nodeStates[replica];
+            var rState' := ss'.nodeStates[replica];
+            LemmaMsgRelationInReplicaNext(rState, inMsg, rState', outMsg);
+        }
+    }
+
+    lemma LemmaReplicaMsgSentIsSubsetOfSystemMsgSentInSystemNextByOneReplica(
+        ss : SystemState, 
+        ss' : SystemState, 
+        replica : Address,
+        inMsg : set<Msg>,
+        outMsg : set<Msg>)
+    requires ValidSystemState(ss)
+    requires inMsg <= ss.msgSent
+    requires SystemNextByOneReplica(ss, ss', replica, inMsg, outMsg)
+    ensures forall r | r in ss'.nodeStates.Keys :: ss'.nodeStates[r].msgSent <= ss'.msgSent
+    {
+        if IsHonest(ss, replica) {
+            var rState := ss.nodeStates[replica];
+            var rState' := ss'.nodeStates[replica];
+            LemmaMsgRelationInReplicaNext(rState, inMsg, rState', outMsg);
+            assert rState'.msgSent <= ss'.msgSent;
+        }
+        else {
+            forall r_byz | r_byz in ss.adversary.byz_nodes
+            ensures ss'.nodeStates[r_byz].msgSent <= ss'.msgSent {
+                var byzState := ss.nodeStates[r_byz];
+                var byzState' := ss'.nodeStates[r_byz];
+                // assert forall r | r in ss.nodeStates.Keys :: ss.nodeStates[r].msgSent <= ss.msgSent by {
+                //     assert ValidSystemState(ss);
+                // }
+                assert byzState'.msgSent <= ss'.msgSent;
+            }
+        }
+    }
+
+    lemma LemmaSystemNextByOneReplicaIsValid(
+        ss : SystemState, 
+        ss' : SystemState, 
+        replica : Address,
+        inMsg : set<Msg>,
+        outMsg : set<Msg>)
+    requires ValidSystemState(ss)
+    requires inMsg <= ss.msgSent
+    requires SystemNextByOneReplica(ss, ss', replica, inMsg, outMsg)
+    ensures ValidSystemState(ss')
+    {
+        LemmaInvNodeInSystemNextByOneReplica(ss, ss', replica, inMsg, outMsg);
+        LemmaReplicaMsgSentIsSubsetOfSystemMsgSentInSystemNextByOneReplica(ss, ss', replica, inMsg, outMsg);
+        LemmaHonestReplicaIsValidInSystemNextByOneReplica(ss, ss', replica, inMsg, outMsg);
+        LemmaHonestReplicaMsgReceivedIsSubsetOfSystemMsgSentInSystemNextByOneReplica(ss, ss', replica, inMsg, outMsg);
+    }
+}
